io/Hist.fst
@@ -2,43 +2,49 @@ module Hist
 
 open FStar.List.Tot.Base
 open Common
+open Free.IO
 
-let trace = Free.IO.trace
+// local_trace (from old to new)
+let hist_post a = a -> lt:trace -> Type0
 
-let hist_post a = r:a -> lt:trace -> Type0
-let hist_pre a = h:trace -> Type0
-
-let hist a = hist_post a -> hist_pre a 
-
-unfold
-let hist_return (x:'a) : hist 'a =
-  fun p _ -> p x []
-
-unfold 
-let hist_shift_post (p:hist_post 'a) (lt:trace) : hist_post 'a =
-  fun r lt' -> p r (lt @ lt')
+// past_events (from new to old; reversed compared with local_trace)
+let hist a = h:trace -> hist_post a -> Type0
 
 unfold
-let hist_post_bind
+let hist_return (a:Type) (x:a) : hist a =
+  fun _ p -> p x []
+
+unfold
+let compute_post
+  (a b:Type)
   (h:trace)
-  (kw : 'a -> hist 'b)
-  (p:hist_post 'b) :
-  Tot (hist_post 'a) =
-  fun r lt ->
-    kw r (hist_shift_post p lt) ((List.rev lt) @ h)
+  (kw : a -> hist b)
+  (p:hist_post b) :
+  Tot (hist_post a) =
+  (fun result local_trace ->
+      kw result
+       ((List.rev local_trace) @ h)
+       (fun result' local_trace' ->
+         p result' (local_trace @ local_trace')))
 
 unfold
-let hist_bind (w : hist 'a) (kw : 'a -> hist 'b) : hist 'b =
-  fun p h -> w (hist_post_bind h kw p) h
+let hist_bind
+  (a:Type)
+  (b:Type)
+  (w : hist a)
+  (kw : a -> hist b) :
+  Tot (hist b) =
+  fun h p ->
+    w h (compute_post a b h kw p)
 
-unfold
-let wp_lift_pure_hist (w : pure_wp 'a) : hist 'a =
-  fun p _ -> w (fun x -> p x [])
+let gen_post #a (post:hist_post a) (cmd:io_cmds) arg res =
+  fun r local_trace ->
+    post r (convert_call_to_event cmd arg res :: local_trace)
 
 unfold
 val hist_ord (#a : Type) : hist a -> hist a -> Type0
-let hist_ord wp1 wp2 = forall h p. wp1 p h ==> wp2 p h
+let hist_ord wp1 wp2 = forall h p. wp1 h p ==> wp2 h p
 
 unfold
-let hist_if_then_else (wp1 wp2:hist 'a) (b:bool) : hist 'a =
-  fun p h -> (b ==> wp1 p h) /\ ((~b) ==> wp2 p h)
+let hist_if_then_else (#a:Type) (wp1 wp2:hist a) (b:bool) : hist a =
+  fun h p -> (b ==> wp1 h p) /\ ((~b) ==> wp2 h p)
